Work on typed circuits defining compose

TypedCircuits.v
@@ -3,7 +3,7 @@ Require Import List.
 Import ListNotations.
 Open Scope list_scope.
 
-Require Import Contexts.
+
 
 Inductive WType := Qubit | Bit | One | Tensor : WType -> WType -> WType.
 
@@ -52,6 +52,23 @@ Inductive MergeCtx : Ctx -> Ctx -> Ctx -> Set :=
 | MergeCons : forall o1 o2 o g1 g2 g, 
               MergeOption o1 o2 o -> MergeCtx g1 g2 g -> MergeCtx (o1 :: g1) (o2 :: g2) (o :: g)
 .
+Fixpoint MergeOptionF (o1 : option WType) (o2 : option WType) 
+         : option (option WType) :=
+  match o1, o2 with
+  | None, _ => Some o2
+  | _, None => Some o1
+  | Some _, Some _ => None
+  end.
+Fixpoint MergeCtxF (Γ1 : Ctx) (Γ2 : Ctx) : option Ctx :=
+  match Γ1, Γ2 with
+  | [], _ => Some Γ2
+  | _, [] => Some Γ1
+  | (o1 :: Γ1'), (o2 :: Γ2') => 
+    match MergeOptionF o1 o2, MergeCtxF Γ1' Γ2' with
+    | Some o, Some Γ => Some (o :: Γ)
+    | _, _           => None
+    end
+  end.
 
 Inductive Pat : Ctx -> WType -> Set :=
 | var  : forall x w ctx, SingletonCtx x w ctx -> Pat ctx w
@@ -84,24 +101,99 @@ Definition unbox {ctx} {w1} {w2} (b : Box w1 w2) : Pat ctx w1 -> Circuit ctx w2 
   match b with
     box f => f ctx
   end.
-
-Fixpoint compose {ctx1} {w} (c : Circuit ctx1 w)
+(*
+Program Fixpoint compose {ctx1} {w} (c : Circuit ctx1 w)
                  : forall {ctx} {ctx1'} {w'}, 
                   (forall ctx2 ctx2', MergeCtx ctx2 ctx ctx2'
                                     -> Pat ctx2 w 
                                     -> Circuit ctx2' w') 
-               -> MergeCtx ctx1 ctx ctx1' -> Circuit ctx1' w'.
+               -> MergeCtx ctx1 ctx ctx1' -> Circuit ctx1' w' :=
+  match c with
+    | output p1 => _
+    | gate ctx g p1 h pfM => _
+  end.
+*)
+
+Lemma mergeF : forall {Γ1 Γ2 Γ}, MergeCtxF Γ1 Γ2 = Some Γ -> MergeCtx Γ1 Γ2 Γ.
+Proof.
+  induction Γ1 as [ | o1 Γ1']; simpl; intros Γ2 Γ H; inversion H; subst; try constructor.
+  destruct Γ2 as [ | o2 Γ2']. inversion H; subst. constructor.
+  destruct o1; destruct o2; simpl in *; try (inversion H1; fail).
+  - remember (MergeCtxF Γ1' Γ2'). 
+    destruct o; simpl in *; try (inversion H1; fail).
+    inversion H; subst. constructor. constructor. apply IHΓ1'; auto.
+  - remember (MergeCtxF Γ1' Γ2'). 
+    destruct o; simpl in *; try (inversion H1; fail).
+    inversion H; subst. constructor. constructor. apply IHΓ1'; auto.
+  - remember (MergeCtxF Γ1' Γ2'). 
+    destruct o; simpl in *; try (inversion H1; fail).
+    inversion H; subst. constructor. constructor. apply IHΓ1'; auto.
+Qed.    
+Open Scope type_scope.
+
+Definition Disjoint Γ1 Γ2 := {Γ : Ctx & MergeCtxF Γ1 Γ2 = Some Γ}.
+Definition Subset Γ1 Γ := {Γ2 : Ctx & MergeCtxF Γ1 Γ2 = Some Γ}.
+
+Lemma mergeDisjoint : forall Γ1 Γ2 Γ3 Γ Γ',
+      MergeCtx Γ1 Γ2 Γ -> MergeCtx Γ Γ3 Γ' -> Disjoint Γ1 Γ3 * Disjoint Γ2 Γ3.
+Admitted.
+
+Lemma disjointTrans : forall Γ1 Γ2 Γ Γ', MergeCtx Γ1 Γ2 Γ -> Disjoint Γ1 Γ' -> Disjoint Γ2 Γ' 
+                      -> Disjoint Γ Γ'.
+Admitted.
+
+Lemma mergeAssoc : forall Γ1 Γ2 Γ3 Γ Γ' Γ0,
+      MergeCtx Γ1 Γ2 Γ -> MergeCtx Γ Γ3 Γ' 
+   -> MergeCtxF Γ2 Γ3 = Some Γ0
+   -> (MergeCtx Γ2 Γ3 Γ0) * (MergeCtx Γ1 Γ0 Γ').
+Admitted.
+
+Lemma mergeSymm : forall {Γ1 Γ2 Γ}, MergeCtx Γ1 Γ2 Γ -> MergeCtx Γ2 Γ1 Γ.
+Admitted.
+
+Fixpoint compose {Γ1} {W} (c : Circuit Γ1 W)
+                 : forall {Γ} {Γ1'} {W'}, 
+                  (forall {Γ2} {Γ2'}, MergeCtx Γ2 Γ Γ2'
+                                    -> Pat Γ2 W
+                                    -> Circuit Γ2' W') 
+               -> MergeCtx Γ1 Γ Γ1' -> Circuit Γ1' W'.
   refine (match c with
-            output p1 => fun _ _ _ f pfM => f _ _ pfM p1
-          | gate ctx g p1 h pfM => _
+            output p1 => fun Γ Γ1' W' f pfM => f _ _ pfM p1
+          | gate ctx g p1 h pfM => fun Γ Γ1' W' f pfM0 => _
           end). 
-  clear w c ctx1; 
-  rename c0 into ctx1, c1 into ctx1', w0 into w1, w1 into w2, w2 into w.
-  intros ctx0 ctx01 w' f pfM'.
-  refine (gate _ g p1 (fun ctx2 ctx2' pfM'' p2 => compose _ _ (h _ _ _ p2) _ _ _ _ _) _).
-    - admit.
-    - intros ctx3 ctx3' pfM3 p3. eapply (f _ _ _ p3).
-    - admit.
-    - admit.
+  clear W c Γ1.
+  rename w into W1, w0 into W2, w1 into W.
+  rename c0 into Γ01, c1 into Γ1, ctx into Γ0.
+  destruct (mergeDisjoint Γ01 Γ0 Γ Γ1 Γ1') as [[Γ01' pfM1] [Γ0' pfM2]]; auto.
+  destruct (mergeAssoc Γ01 Γ0 Γ Γ1 Γ1' Γ0') as [pfM3 pfM4]; auto.
+  refine (gate _ g p1 (fun Γ02 Γ02' pfM' q => _) pfM4);
+    destruct (mergeDisjoint Γ0 Γ Γ02 Γ0' Γ02') as [[Γ002 pfM6] [Γ02'' pfM5]];
+      try (auto; apply mergeSymm; auto).
+  refine (compose _ _ (h Γ02 Γ002 _ q) _ _ _ f _).
+  - apply mergeSymm. apply mergeF. apply pfM6.
+  - (* Γ002 = Γ0 ⋓ Γ02 *)
+    (* Γ02' = Γ02 ⋓ Γ0' = Γ02 ⋓ (Γ0 ⋓ Γ) *)
+    (* So want to show that (Γ0 ⋓ Γ02) ⋓ Γ = Γ02 ⋓ (Γ0 ⋓ Γ) *)
+    (* First show that (Γ02 ⋓ Γ0) ⋓ Γ = Γ02 ⋓ (Γ0 ⋓ Γ) *)
+    (* Before that, show that Γ002 _|_ Γ *)
+    (* To do that, show that Γ0 _|_ Γ*) 
+    assert (pfDisjoint1 : Disjoint Γ0 Γ).
+      exists Γ0'; auto.
+    assert (pfDisjoint2 : Disjoint Γ02 Γ).
+      admit.
+    assert (pfDisjoint3 : Disjoint Γ002 Γ).
+      apply disjointTrans with (Γ1 := Γ0) (Γ2 := Γ02); auto. apply mergeF; auto.
+    destruct pfDisjoint1 as [ Γ0001 pfDisjoint1].
+    destruct pfDisjoint3 as [ Γ0002 pfDisjoint3]. 
+    (* as a result of mergeAssoc, we want Γ002 ⋓ Γ = Γ02' *)
+
+    edestruct (mergeAssoc Γ02 Γ0 Γ).
+    * eapply mergeSymm. eapply mergeF. eauto. 
+    * eapply mergeF. exact pfDisjoint3.
+    * exact pfDisjoint1.
+    * 
+    
+
+
 Admitted.
 
